Classes/Except.v
@@ -5,13 +5,10 @@ Require Import Classes.Monad.
 Class Except (M : Type -> Type) `{Monad M} := {
   throw    : forall {A}, M A;
   trycatch : forall {A}, M A -> M A -> M A;
-  bind_fail : forall {A} (f : unit -> M A), bindM throw f = throw;
   trycatch_throw_left : forall {A} (x : M A), 
     trycatch throw x = x;
   trycatch_throw_right : forall {A} (x : M A),
     trycatch x throw = x;
-  trycatch_pure : forall {A} x h, trycatch (pure x) h = pure (A:=A) x;
 }.
 
-Hint Rewrite @trycatch_throw_left @trycatch_throw_right 
-  @trycatch_pure : soundness.
+Hint Rewrite @trycatch_throw_left @trycatch_throw_right : soundness.
